remove Hacl.Bignum

code/experimental/curve25519_64/Hacl.Bignum.Fdifference.fst
@@ -8,9 +8,12 @@ open FStar.HyperStack
 open FStar.Buffer
 
 open Hacl.Bignum.Parameters
-open Hacl.Spec.Bignum.Bigint
+open Hacl.Bignum.Modulo
 open Hacl.Bignum.Limb
+open Hacl.Spec.Bignum
+open Hacl.Spec.Bignum.Bigint
 open Hacl.Spec.Bignum.Fdifference
+open Hacl.Spec.Bignum.Modulo
 
 #reset-options "--max_fuel 0 --max_ifuel 0 --z3rlimit 20"
 
@@ -29,3 +32,47 @@ val fdifference_:
 [@"substitute"]
 let rec fdifference_ a b =
   C.Loops.in_place_map2 a b clen (fun x y -> y -%^ x)
+
+assume val lemma_diff: a:int -> b:int -> p:pos ->
+  Lemma ( (a - b) % p = ((a%p) - b) % p /\ (a - b) % p = (a - (b % p)) % p)
+  
+#reset-options "--z3rlimit 100 --max_fuel 0 --max_ifuel 0"
+
+[@"c_inline"]
+val fdifference:
+  a:felem ->
+  b:felem{disjoint a b} ->
+  Stack unit
+    (requires (fun h -> live h a /\ live h b /\ add_zero_pre (as_seq h b)
+      /\ Hacl.Spec.Bignum.Fdifference.gte_limbs (as_seq h a) (add_zero_spec (as_seq h b)) len))
+    (ensures (fun h0 _ h1 -> live h0 a /\ live h0 b
+      /\ live h1 a /\ modifies_1 a h0 h1
+      /\ add_zero_pre (as_seq h0 b)
+      /\ Hacl.Spec.Bignum.Fdifference.gte_limbs (as_seq h0 a) (add_zero_spec (as_seq h0 b)) len
+      /\ eval h1 a % prime = (eval h0 b - eval h0 a) % prime
+      /\ as_seq h1 a == fdifference_tot (as_seq h0 a) (as_seq h0 b)
+      ))
+[@"c_inline"]
+let fdifference a b =
+  let hinit = ST.get() in
+  push_frame();
+  let h0 = ST.get() in
+  let tmp = create limb_zero clen in
+  let h0' = ST.get() in
+  blit b 0ul tmp 0ul clen;
+  let h = ST.get() in
+  Hacl.Spec.Bignum.Fmul.lemma_whole_slice (as_seq h b);
+  Hacl.Spec.Bignum.Fmul.lemma_whole_slice (as_seq h tmp);
+  FStar.Seq.lemma_eq_intro (as_seq h b) (as_seq h tmp);
+  add_zero tmp;
+  let h' = ST.get() in
+  cut (eval h' tmp % prime = eval hinit b % prime);
+  fdifference_ a tmp;
+  let h1 = ST.get() in
+  Hacl.Spec.Bignum.Fdifference.lemma_fdifference_eval (as_seq hinit a) (as_seq h' tmp);
+  lemma_diff (eval h' tmp) (eval hinit a) prime;
+  lemma_diff (eval hinit b) (eval hinit a) prime;
+  pop_frame();
+  lemma_modifies_1_trans tmp h0' h h';
+  lemma_modifies_0_1' tmp h0 h0' h';
+  lemma_modifies_0_1 a h0 h' h1
